Rework modules: types

theories/Syntax/Types.v
@@ -32,88 +32,34 @@ From Coq Require Import
      ZArith.ZArith.
 From bbv Require
      Word.
-From stdpp Require
-     finite.
 From Equations Require Import
      Equations.
 From Katamaran Require Export
-     Context
      Environment
      Prelude
-     Tactics.
+     Tactics
+     Syntax.TypeKit
+     Syntax.Variables.
+
+Import ctx.notations.
 
 Local Set Implicit Arguments.
-Local Unset Transparent Obligations.
-Obligation Tactic := idtac.
+Local Set Transparent Obligations.
+Local Unset Elimination Schemes.
 
-Module Type EnumTypeKit.
-  (* Names of enum type constructors. *)
-  Parameter Inline 𝑬 : Set. (* input: \MIE *)
-  Declare Instance 𝑬_eq_dec : EqDec 𝑬.
-  (* Names of enum data constructors. *)
-  Parameter Inline 𝑬𝑲 : 𝑬 -> Set.
-  Declare Instance 𝑬𝑲_eq_dec : forall (e : 𝑬), EqDec (𝑬𝑲 e).
-  Declare Instance 𝑬𝑲_finite : forall E, finite.Finite (𝑬𝑲 E).
-End EnumTypeKit.
+Inductive Bit : Set := bitzero | bitone.
 
-Module Type UnionTypeKit.
-  (* Names of union type constructors. *)
-  Parameter Inline 𝑼   : Set. (* input: \MIU *)
-  Declare Instance 𝑼_eq_dec : EqDec 𝑼.
-  (* Union types. *)
-  Parameter Inline 𝑼𝑻  : 𝑼 -> Set.
-  Declare Instance 𝑼𝑻_eq_dec : forall (u : 𝑼), EqDec (𝑼𝑻 u).
-  (* Names of union data constructors. *)
-  Parameter Inline 𝑼𝑲  : 𝑼 -> Set.
-  Declare Instance 𝑼𝑲_eq_dec : forall (u : 𝑼), EqDec (𝑼𝑲 u).
-  Declare Instance 𝑼𝑲_finite : forall U, finite.Finite (𝑼𝑲 U).
-End UnionTypeKit.
+Definition Bit_eqb (b1 : Bit) (b2 : Bit) : bool :=
+  match b1, b2 with
+  | bitzero, bitzero => true
+  | bitone , bitone  => true
+  | _      , _       => false
+  end.
 
-Module Type RecordTypeKit.
-  (* Names of record type constructors. *)
-  Parameter Inline 𝑹  : Set. (* input: \MIR *)
-  Declare Instance 𝑹_eq_dec : EqDec 𝑹.
-  (* Record types. *)
-  Parameter Inline 𝑹𝑻  : 𝑹 -> Set.
-  Declare Instance 𝑹𝑻_eq_dec : forall (r : 𝑹), EqDec (𝑹𝑻 r).
-End RecordTypeKit.
+Lemma Bit_eqb_spec (b1 b2 : Bit) : reflect (b1 = b2) (Bit_eqb b1 b2).
+Proof. destruct b1, b2; cbn; constructor; congruence. Qed.
 
-Module Type TypeKit :=
-  EnumTypeKit <+ UnionTypeKit <+ RecordTypeKit.
-
-Module NoEnums <: EnumTypeKit.
-  Definition 𝑬          := Empty_set.
-  Definition 𝑬𝑲 (E : 𝑬) := Empty_set.
-
-  Instance 𝑬_eq_dec : EqDec 𝑬 := Empty_set_EqDec.
-  Instance 𝑬𝑲_eq_dec (E : 𝑬) : EqDec (𝑬𝑲 E)  := Empty_set_EqDec.
-  Instance 𝑬𝑲_finite (E : 𝑬) : finite.Finite (𝑬𝑲 E) := finite.Empty_set_finite.
-End NoEnums.
-
-Module NoUnions <: UnionTypeKit.
-  Definition 𝑼          := Empty_set.
-  Definition 𝑼𝑻 (U : 𝑼) := Empty_set.
-  Definition 𝑼𝑲 (U : 𝑼) := Empty_set.
-
-  Instance 𝑼_eq_dec : EqDec 𝑼 := Empty_set_EqDec.
-  Instance 𝑼𝑻_eq_dec (U : 𝑼) : EqDec (𝑼𝑻 U)  := Empty_set_EqDec.
-  Instance 𝑼𝑲_eq_dec (U : 𝑼) : EqDec (𝑼𝑲 U)  := Empty_set_EqDec.
-  Instance 𝑼𝑲_finite (U : 𝑼) : finite.Finite (𝑼𝑲 U) := finite.Empty_set_finite.
-End NoUnions.
-
-Module NoRecords <: RecordTypeKit.
-  Definition 𝑹          := Empty_set.
-  Definition 𝑹𝑻 (R : 𝑹) := Empty_set.
-  Instance 𝑹_eq_dec : EqDec 𝑹 := Empty_set_EqDec.
-  Instance 𝑹𝑻_eq_dec (R : 𝑹) : EqDec (𝑹𝑻 R) := Empty_set_EqDec.
-End NoRecords.
-
-Module DefaultTypeKit <: TypeKit := NoEnums <+ NoUnions <+ NoRecords.
-
-Module Types (Export typekit : TypeKit).
-
-  Local Set Transparent Obligations.
-  Local Unset Elimination Schemes.
+Module Type TypeCodeOn (Import typekit : TypeKit).
 
   Inductive Ty : Set :=
   | ty_int
@@ -126,7 +72,6 @@ Module Types (Export typekit : TypeKit).
   | ty_unit
   | ty_enum (E : 𝑬)
   | ty_bvec (n : nat)
-  (* Experimental features. These are still in flux. *)
   | ty_tuple (σs : Ctx Ty)
   | ty_union (U : 𝑼)
   | ty_record (R : 𝑹)
@@ -176,7 +121,7 @@ Module Types (Export typekit : TypeKit).
   Definition Ty_rec (P : Ty -> Set) := Ty_rect P.
   Definition Ty_ind (P : Ty -> Prop) := Ty_rect P.
 
-  Global Instance Ty_eq_dec : EqDec Ty :=
+  Instance Ty_eq_dec : EqDec Ty :=
     fix ty_eqdec (σ τ : Ty) {struct σ} : dec_eq σ τ :=
       match σ , τ with
       | ty_int        , ty_int        => left eq_refl
@@ -189,26 +134,20 @@ Module Types (Export typekit : TypeKit).
       | ty_unit       , ty_unit       => left eq_refl
       | ty_enum E1    , ty_enum E2    => f_equal_dec ty_enum noConfusion_inv (eq_dec E1 E2)
       | ty_bvec n1    , ty_bvec n2    => f_equal_dec ty_bvec noConfusion_inv (eq_dec n1 n2)
-      | ty_tuple σs   , ty_tuple τs   => f_equal_dec ty_tuple noConfusion_inv (eq_dec (EqDec := ctx.eq_dec_ctx ty_eqdec) σs τs)
+      | ty_tuple σs   , ty_tuple τs   => f_equal_dec
+                                           ty_tuple noConfusion_inv
+                                           (eq_dec (EqDec := ctx.eq_dec_ctx ty_eqdec) σs τs)
       | ty_union U1   , ty_union U2   => f_equal_dec ty_union noConfusion_inv (eq_dec U1 U2)
       | ty_record R1  , ty_record R2  => f_equal_dec ty_record noConfusion_inv (eq_dec R1 R2)
       | _             , _             => right noConfusion_inv
       end.
 
-  Lemma Ty_K (σ : Ty) (p : σ = σ) : p = eq_refl.
-  Proof. apply uip. Qed.
+  (* Lemma Ty_K (σ : Ty) (p : σ = σ) : p = eq_refl. *)
+  (* Proof. apply uip. Qed. *)
 
-  Inductive Bit : Set := bitzero | bitone.
+End TypeCodeOn.
 
-  Definition Bit_eqb (b1 : Bit) (b2 : Bit) : bool :=
-    match b1, b2 with
-    | bitzero, bitzero => true
-    | bitone , bitone  => true
-    | _      , _       => false
-    end.
-
-  Lemma Bit_eqb_spec (b1 b2 : Bit) : reflect (b1 = b2) (Bit_eqb b1 b2).
-  Proof. destruct b1, b2; cbn; constructor; congruence. Qed.
+Module Type TypeExtOn (Import TK : TypeKit) (Import TY : TypeCodeOn TK).
 
   Fixpoint Val (σ : Ty) : Set :=
     match σ with
@@ -222,11 +161,219 @@ Module Types (Export typekit : TypeKit).
     | ty_unit => unit
     | ty_enum E => 𝑬𝑲 E
     | ty_bvec n => Word.word n
-    (* Experimental features *)
     | ty_tuple σs => EnvRec Val σs
     | ty_union U => 𝑼𝑻 U
     | ty_record R => 𝑹𝑻 R
     end%type.
   Bind Scope exp_scope with Val.
 
+  Fixpoint Val_eqb (σ : Ty) : forall (l1 l2 : Val σ), bool :=
+    match σ return Val σ -> Val σ -> bool with
+    | ty_int      => Z.eqb
+    | ty_bool     => Bool.eqb
+    | ty_bit      => Bit_eqb
+    | ty_string   => String.eqb
+    | ty_list σ   => list_beq (Val_eqb σ)
+    | ty_prod σ τ => prod_beq (Val_eqb σ) (Val_eqb τ)
+    | ty_sum σ τ  => sum_beq (Val_eqb σ) (Val_eqb τ)
+    | ty_unit     => fun _ _ => true
+    | ty_enum E   => fun l1 l2 => if eq_dec l1 l2 then true else false
+    | ty_bvec n   => @Word.weqb n
+    | ty_tuple σs => envrec.eqb Val_eqb
+    | ty_union U  => fun l1 l2 => if eq_dec l1 l2 then true else false
+    | ty_record R => fun l1 l2 => if eq_dec l1 l2 then true else false
+    end.
+
+  Lemma Val_eqb_spec (σ : Ty) (x y : Val σ) : reflect (x = y) (Val_eqb σ x y).
+  Proof with solve_eqb_spec.
+    induction σ; cbn.
+    - apply Z.eqb_spec.
+    - apply Bool.eqb_spec.
+    - apply Bit_eqb_spec.
+    - apply String.eqb_spec.
+    - apply list_beq_spec; auto.
+    - destruct x as [x1 x2]; destruct y as [y1 y2]...
+    - destruct x as [x1|x2]; destruct y as [y1|y2]...
+    - destruct x. destruct y...
+    - destruct (eq_dec x y)...
+    - apply iff_reflect. symmetry.
+      apply (Word.weqb_true_iff x y).
+    - induction σs; intros.
+      + destruct x; destruct y...
+      + cbn in *.
+        destruct x as [xs x]; destruct y as [ys y]; destruct X as [pσs pb]; cbn in *.
+        specialize (IHσs pσs).
+        destruct (IHσs xs ys); destruct (pb x y)...
+    - destruct (eq_dec x y)...
+    - destruct (eq_dec x y)...
+  Qed.
+
+  (* TODO: deprecate tuple projections *)
+  Fixpoint tuple_proj (σs : Ctx Ty) (n : nat) (σ : Ty) :
+    Val (ty_tuple σs) -> ctx.nth_is σs n σ -> Val σ :=
+    match σs with
+    | ctx.nil =>
+        fun l (p : ctx.nth_is ctx.nil _ _) =>
+          match p with end
+    | ctx.snoc τs τ =>
+        match n with
+        | 0   => fun (l : Val (ty_tuple (ctx.snoc _ _)))
+                     (p : ctx.nth_is _ 0 _) =>
+                   @eq_rect Ty τ Val (snd l) σ p
+        | S m => fun l p => tuple_proj τs m σ (fst l) p
+        end
+    end.
+
+End TypeExtOn.
+
+Module Type BinopsOn (Import TK : TypeKit) (Import TY : TypeCodeOn TK).
+
+  Inductive BinOp : Ty -> Ty -> Ty -> Set :=
+  | binop_plus              : BinOp ty_int ty_int ty_int
+  | binop_times             : BinOp ty_int ty_int ty_int
+  | binop_minus             : BinOp ty_int ty_int ty_int
+  | binop_eq                : BinOp ty_int ty_int ty_bool
+  | binop_le                : BinOp ty_int ty_int ty_bool
+  | binop_lt                : BinOp ty_int ty_int ty_bool
+  | binop_ge                : BinOp ty_int ty_int ty_bool
+  | binop_gt                : BinOp ty_int ty_int ty_bool
+  | binop_and               : BinOp ty_bool ty_bool ty_bool
+  | binop_or                : BinOp ty_bool ty_bool ty_bool
+  | binop_pair {σ1 σ2 : Ty} : BinOp σ1 σ2 (ty_prod σ1 σ2)
+  | binop_cons {σ : Ty}     : BinOp σ (ty_list σ) (ty_list σ)
+  | binop_append {σ : Ty}   : BinOp (ty_list σ) (ty_list σ) (ty_list σ)
+  | binop_tuple_snoc {σs σ} : BinOp (ty_tuple σs) σ (ty_tuple (σs ▻ σ))
+  | binop_bvplus {n}        : BinOp (ty_bvec n) (ty_bvec n) (ty_bvec n)
+  | binop_bvmult {n}        : BinOp (ty_bvec n) (ty_bvec n) (ty_bvec n)
+  | binop_bvcombine {m n}   : BinOp (ty_bvec m) (ty_bvec n) (ty_bvec (m + n))
+  | binop_bvcons {m}        : BinOp (ty_bit) (ty_bvec m) (ty_bvec (S m))
+  .
+
+  Derive Signature NoConfusion for BinOp.
+
+  Import Sigma_Notations.
+
+  Definition BinOpTel : Set :=
+    Σ i : (Σ σ1 σ2 : Ty, Ty), BinOp i.1 (i.2).1 (i.2).2.
+
+  Definition binoptel_pair (σ1 σ2 : Ty) : BinOpTel :=
+    ((σ1, σ2, ty_prod σ1 σ2), binop_pair).
+  Definition binoptel_cons (σ : Ty) : BinOpTel :=
+    ((σ, ty_list σ, ty_list σ), binop_cons).
+  Definition binoptel_append (σ : Ty) : BinOpTel :=
+    ((ty_list σ, ty_list σ, ty_list σ), binop_append).
+  Definition binoptel_tuple_snoc (σs : Ctx Ty) (σ : Ty) : BinOpTel :=
+    ((ty_tuple σs, σ, ty_tuple (σs ▻ σ)), binop_tuple_snoc).
+
+  Definition binoptel_eq_dec {σ1 σ2 σ3 τ1 τ2 τ3}
+    (op1 : BinOp σ1 σ2 σ3) (op2 : BinOp τ1 τ2 τ3) :
+    dec_eq (A := BinOpTel) ((σ1,σ2,σ3),op1) ((τ1,τ2,τ3),op2) :=
+    match op1 , op2 with
+    | binop_plus  , binop_plus   => left eq_refl
+    | binop_times , binop_times  => left eq_refl
+    | binop_minus , binop_minus  => left eq_refl
+    | binop_eq    , binop_eq     => left eq_refl
+    | binop_le    , binop_le     => left eq_refl
+    | binop_lt    , binop_lt     => left eq_refl
+    | binop_ge    , binop_ge     => left eq_refl
+    | binop_gt    , binop_gt     => left eq_refl
+    | binop_and   , binop_and    => left eq_refl
+    | binop_or    , binop_or     => left eq_refl
+    | @binop_pair σ1 σ2 , @binop_pair τ1 τ2   =>
+      f_equal2_dec binoptel_pair noConfusion_inv (eq_dec σ1 τ1) (eq_dec σ2 τ2)
+    | @binop_cons σ  , @binop_cons τ   =>
+      f_equal_dec binoptel_cons noConfusion_inv (eq_dec σ τ)
+    | @binop_append σ , @binop_append τ   =>
+      f_equal_dec binoptel_append noConfusion_inv (eq_dec σ τ)
+    | @binop_tuple_snoc σs σ , @binop_tuple_snoc τs τ =>
+      f_equal2_dec binoptel_tuple_snoc noConfusion_inv (eq_dec σs τs) (eq_dec σ τ)
+    | @binop_bvplus m , @binop_bvplus n =>
+      f_equal_dec
+        (fun n => ((ty_bvec n, ty_bvec n, ty_bvec n), binop_bvplus))
+        noConfusion_inv (eq_dec m n)
+    | @binop_bvmult m , @binop_bvmult n =>
+      f_equal_dec
+        (fun n => ((ty_bvec n, ty_bvec n, ty_bvec n), binop_bvmult))
+        noConfusion_inv (eq_dec m n)
+    | @binop_bvcombine m1 m2 , @binop_bvcombine n1 n2 =>
+      f_equal2_dec
+        (fun m n => ((ty_bvec m, ty_bvec n, ty_bvec (m+n)), binop_bvcombine))
+        noConfusion_inv (eq_dec m1 n1) (eq_dec m2 n2)
+    | @binop_bvcons m , @binop_bvcons n =>
+      f_equal_dec
+        (fun n => ((ty_bit, ty_bvec n, ty_bvec (S n)), binop_bvcons))
+        noConfusion_inv (eq_dec m n)
+    | _           , _            => right noConfusion_inv
+    end.
+
+  Inductive OpEq {σ1 σ2 σ3} (op1 : BinOp σ1 σ2 σ3) : forall τ1 τ2 τ3, BinOp τ1 τ2 τ3 -> Prop :=
+  | opeq_refl : OpEq op1 op1.
+  Derive Signature for OpEq.
+  Global Arguments opeq_refl {_ _ _ _}.
+
+  Lemma binop_eqdep_dec {σ1 σ2 σ3 τ1 τ2 τ3} (op1 : BinOp σ1 σ2 σ3) (op2 : BinOp τ1 τ2 τ3) :
+    {OpEq op1 op2} + {~ OpEq op1 op2}.
+  Proof.
+    destruct (binoptel_eq_dec op1 op2).
+    - left. dependent elimination e. constructor.
+    - right. intro e. apply n. dependent elimination e. reflexivity.
+  Defined.
+
+  Local Set Equations With UIP.
+  Instance binop_eq_dec {σ1 σ2 σ3} : EqDec (BinOp σ1 σ2 σ3).
+  Proof.
+    intros x y.
+    destruct (binoptel_eq_dec x y) as [p|p].
+    - left. dependent elimination p. reflexivity.
+    - right. congruence.
+  Defined.
+
+End BinopsOn.
+
+Module Type BinopEvalOn (Import TK  : TypeKit) (Import TY  : TypeCodeOn TK)
+       (Import LIT : TypeExtOn TK TY) (Import BOP : BinopsOn TK TY).
+
+  Definition eval_binop {σ1 σ2 σ3 : Ty} (op : BinOp σ1 σ2 σ3) : Val σ1 -> Val σ2 -> Val σ3 :=
+    match op with
+    | binop_plus       => Z.add
+    | binop_times      => Z.mul
+    | binop_minus      => Z.sub
+    | binop_eq         => Z.eqb
+    | binop_le         => Z.leb
+    | binop_lt         => Z.ltb
+    | binop_ge         => Z.geb
+    | binop_gt         => Z.gtb
+    | binop_and        => andb
+    | binop_or         => fun v1 v2 => orb v1 v2
+    | binop_pair       => pair
+    | binop_cons       => cons
+    | binop_append     => app
+    | binop_tuple_snoc => pair
+    | binop_bvplus     => fun v1 v2 => Word.wplus v1 v2
+    | binop_bvmult     => fun v1 v2 => Word.wmult v1 v2
+    | binop_bvcombine  => fun v1 v2 => Word.combine v1 v2
+    | binop_bvcons     => fun b bs => Word.WS (Bit_eqb b bitone) bs
+    end.
+
+End BinopEvalOn.
+
+Module Type TypesOn (TK : TypeKit) :=
+  TypeCodeOn TK <+ TypeExtOn TK <+ BinopsOn TK <+ BinopEvalOn TK.
+
+Module Type Types.
+  Declare Module Export VAR : VarKit.
+  Declare Module Export TK : TypeKit.TypeKit.
+  Include TypeCodeOn TK <+ TypeExtOn TK <+ BinopsOn TK <+ BinopEvalOn TK.
+
+  Notation PCtx := (NCtx 𝑿 Ty).
+  Notation LCtx := (NCtx 𝑺 Ty).
 End Types.
+
+Module MakeTypes (Export VAR' : VarKit) (Export TK' : TypeKit) <: Types. (* with Module TK := TK'. *)
+  Module VAR := VAR'.
+  Module TK := TK'.
+  Include TypeCodeOn TK <+ TypeExtOn TK <+ BinopsOn TK <+ BinopEvalOn TK.
+
+  Notation PCtx := (NCtx 𝑿 Ty).
+  Notation LCtx := (NCtx 𝑺 Ty).
+End MakeTypes.
