theories/Syntax/TypeKit.v
@@ -1,0 +1,99 @@
+(******************************************************************************)
+(* Copyright (c) 2019 Steven Keuchel                                          *)
+(* All rights reserved.                                                       *)
+(*                                                                            *)
+(* Redistribution and use in source and binary forms, with or without         *)
+(* modification, are permitted provided that the following conditions are     *)
+(* met:                                                                       *)
+(*                                                                            *)
+(* 1. Redistributions of source code must retain the above copyright notice,  *)
+(*    this list of conditions and the following disclaimer.                   *)
+(*                                                                            *)
+(* 2. Redistributions in binary form must reproduce the above copyright       *)
+(*    notice, this list of conditions and the following disclaimer in the     *)
+(*    documentation and/or other materials provided with the distribution.    *)
+(*                                                                            *)
+(* THIS SOFTWARE IS PROVIDED BY THE COPYRIGHT HOLDERS AND CONTRIBUTORS        *)
+(* "AS IS" AND ANY EXPRESS OR IMPLIED WARRANTIES, INCLUDING, BUT NOT LIMITED  *)
+(* TO, THE IMPLIED WARRANTIES OF MERCHANTABILITY AND FITNESS FOR A PARTICULAR *)
+(* PURPOSE ARE DISCLAIMED. IN NO EVENT SHALL THE COPYRIGHT HOLDER OR          *)
+(* CONTRIBUTORS BE LIABLE FOR ANY DIRECT, INDIRECT, INCIDENTAL, SPECIAL,      *)
+(* EXEMPLARY, OR CONSEQUENTIAL DAMAGES (INCLUDING, BUT NOT LIMITED TO,        *)
+(* PROCUREMENT OF SUBSTITUTE GOODS OR SERVICES; LOSS OF USE, DATA, OR         *)
+(* PROFITS; OR BUSINESS INTERRUPTION) HOWEVER CAUSED AND ON ANY THEORY OF     *)
+(* LIABILITY, WHETHER IN CONTRACT, STRICT LIABILITY, OR TORT (INCLUDING       *)
+(* NEGLIGENCE OR OTHERWISE) ARISING IN ANY WAY OUT OF THE USE OF THIS         *)
+(* SOFTWARE, EVEN IF ADVISED OF THE POSSIBILITY OF SUCH DAMAGE.               *)
+(******************************************************************************)
+
+From stdpp Require
+     finite.
+From Equations Require Import
+     Equations.
+From Katamaran Require Export
+     Prelude Tactics.
+
+Module Type EnumTypeKit.
+  (* Names of enum type constructors. *)
+  Parameter Inline 𝑬 : Set. (* input: \MIE *)
+  Declare Instance 𝑬_eq_dec : EqDec 𝑬.
+  (* Names of enum data constructors. *)
+  Parameter Inline 𝑬𝑲 : 𝑬 -> Set.
+  Declare Instance 𝑬𝑲_eq_dec : forall (e : 𝑬), EqDec (𝑬𝑲 e).
+  Declare Instance 𝑬𝑲_finite : forall E, finite.Finite (𝑬𝑲 E).
+End EnumTypeKit.
+
+Module Type UnionTypeKit.
+  (* Names of union type constructors. *)
+  Parameter Inline 𝑼   : Set. (* input: \MIU *)
+  Declare Instance 𝑼_eq_dec : EqDec 𝑼.
+  (* Union types. *)
+  Parameter Inline 𝑼𝑻  : 𝑼 -> Set.
+  Declare Instance 𝑼𝑻_eq_dec : forall (u : 𝑼), EqDec (𝑼𝑻 u).
+  (* Names of union data constructors. *)
+  Parameter Inline 𝑼𝑲  : 𝑼 -> Set.
+  Declare Instance 𝑼𝑲_eq_dec : forall (u : 𝑼), EqDec (𝑼𝑲 u).
+  Declare Instance 𝑼𝑲_finite : forall U, finite.Finite (𝑼𝑲 U).
+End UnionTypeKit.
+
+Module Type RecordTypeKit.
+  (* Names of record type constructors. *)
+  Parameter Inline 𝑹  : Set. (* input: \MIR *)
+  Declare Instance 𝑹_eq_dec : EqDec 𝑹.
+  (* Record types. *)
+  Parameter Inline 𝑹𝑻  : 𝑹 -> Set.
+  Declare Instance 𝑹𝑻_eq_dec : forall (r : 𝑹), EqDec (𝑹𝑻 r).
+End RecordTypeKit.
+
+Module Type TypeKit :=
+  EnumTypeKit <+ UnionTypeKit <+ RecordTypeKit.
+
+Module NoEnums <: EnumTypeKit.
+  Definition 𝑬          := Empty_set.
+  Definition 𝑬𝑲 (E : 𝑬) := Empty_set.
+
+  Instance 𝑬_eq_dec : EqDec 𝑬 := Empty_set_EqDec.
+  Instance 𝑬𝑲_eq_dec (E : 𝑬) : EqDec (𝑬𝑲 E)  := Empty_set_EqDec.
+  Instance 𝑬𝑲_finite (E : 𝑬) : finite.Finite (𝑬𝑲 E) := finite.Empty_set_finite.
+End NoEnums.
+
+Module NoUnions <: UnionTypeKit.
+  Definition 𝑼          := Empty_set.
+  Definition 𝑼𝑻 (U : 𝑼) := Empty_set.
+  Definition 𝑼𝑲 (U : 𝑼) := Empty_set.
+
+  Instance 𝑼_eq_dec : EqDec 𝑼 := Empty_set_EqDec.
+  Instance 𝑼𝑻_eq_dec (U : 𝑼) : EqDec (𝑼𝑻 U)  := Empty_set_EqDec.
+  Instance 𝑼𝑲_eq_dec (U : 𝑼) : EqDec (𝑼𝑲 U)  := Empty_set_EqDec.
+  Instance 𝑼𝑲_finite (U : 𝑼) : finite.Finite (𝑼𝑲 U) := finite.Empty_set_finite.
+End NoUnions.
+
+Module NoRecords <: RecordTypeKit.
+  Definition 𝑹          := Empty_set.
+  Definition 𝑹𝑻 (R : 𝑹) := Empty_set.
+  Instance 𝑹_eq_dec : EqDec 𝑹 := Empty_set_EqDec.
+  Instance 𝑹𝑻_eq_dec (R : 𝑹) : EqDec (𝑹𝑻 R) := Empty_set_EqDec.
+End NoRecords.
+
+Module DefaultTypeKit <: TypeKit :=
+  NoEnums <+ NoUnions <+ NoRecords.
